ironfleet/src/Dafny/Distributed/Protocol/LiveSHT/RefinementProof/SchedulerRefinement.i.dfy
@@ -29,7 +29,7 @@ lemma Lemma_HostRefinementForPacketsAppliesToIos(
     host:Host,
     host':Host,
     receives:set<Packet>,
-    sends:set<Packet>,
+    sent_packets:seq<LSHTPacket>,
     environment:LSHTEnvironment,
     environment':LSHTEnvironment,
     ios:seq<LSHTIo>
@@ -37,12 +37,12 @@ lemma Lemma_HostRefinementForPacketsAppliesToIos(
     requires LEnvironment_Next(environment, environment');
     requires environment.nextStep == LEnvStepHostIos(host.me, ios);
     requires receives <= PacketsTo(LSHTEnvironment_Refine(environment), host.me);
-    requires sends == LSHTPacketSet_Refine(set io | io in ios && io.LIoOpSend? :: io.s);
-    requires Host_Next(host, host', receives, sends);
+    requires forall p :: p in sent_packets <==> p in (set io | io in ios && io.LIoOpSend? :: io.s);
+    requires Host_Next(host, host', receives, ExtractPacketsFromLSHTPackets(sent_packets));
     ensures  Host_Next(host, host', PacketsTo(LSHTEnvironment_Refine(environment), host.me), LSHTIoSeq_RefineAsSends(ios));
 {
     assert receives <= PacketsTo(LSHTEnvironment_Refine(environment), host.me);
-    assert sends == LSHTIoSeq_RefineAsSends(ios);
+    assert ExtractPacketsFromLSHTPackets(sent_packets) == LSHTIoSeq_RefineAsSends(ios);
 }
 
 predicate LScheduler_RefinementInvariant(s:LScheduler)
